\documentclass{article}

\usepackage[utf8]{inputenc}
\usepackage[english]{babel}
\usepackage[margin=1in]{geometry} 
\usepackage{amsmath,amsthm,amssymb,hyperref}
\usepackage{graphicx}
\graphicspath{ {./Resources/} }

\begin{document}


\title{Homework Assingment }
\author{Evan Leonov\\Complex Analysis} 

\maketitle

\paragraph{\textbf{Problem 1}} Evaluate the integral 
\[\oint\limits_{C}\mathrm{\frac{e^z}{(z-i)^2\cdot(z+2)}dz}\]

\begin{enumerate}
\item given \(C=C_1: |\mathrm{z-i} |=2\)
\item given \(C=C_2: \mathrm{|z+2-i|}=3\) 
\end{enumerate}

\textbf{Solution: }
	Firstly, we find roots of the denominator of the integrand:
\[\mathrm{(z-i)^2\cdot(z+2)}  = 0 \rightarrow  \mathrm{z=i}\;and\:\mathrm{z=-2}\]

\begin{center}
\includegraphics[scale=0.5]{plot1}
\end{center}

1. A disk \(\mathrm{D} := \{z : |z-i|  < 2\}\) containts only one of the roots (\(z = i\)), therefore we can calculate the integral as usual:

\[\oint\limits_{C_1}\mathrm{\frac{e^z}{(z-i)^2\cdot(z+2)}dz} = \oint\limits_{\mathrm{|z-i|}=2}\mathrm{\frac{e^z}{(z-i)^2\cdot(z+2)}dz} = [\frac{e^z}{(z-i)^2\cdot(z+2)}=\frac{\frac{e^z}{z+2}}{(z-i)^2}]==\oint\limits_{\mathrm{|z-i|}=2}\mathrm{\frac{\frac{e^z}{z+2}}{(z-i)^2}dz}\]

Using Cauchy's Integral Formula for derivatives we evaluate the integral:


\[\oint\limits_{\mathrm{|z-i|}=2}\mathrm{\frac{\frac{e^z}{z+2}}{(z-i)^2}dz }= \frac{2 \pi i}{1!}\cdot (\frac{e^z}{z+2})'|_{\mathrm{z=i}}=2 \pi i \cdot \frac{e^z\cdot (z+1)}{(z+2)^2}|_{\mathrm{z=i}}=2 \pi i \cdot \frac{e^i\cdot (i+1)}{(i+2)^2}\]


2. A disk \(\mathrm{D} := \{z : \mathrm{|z+2-i|}<3\}\) containts both of the roots (\(z = i\; and \;z=-2\)) hence we will evaluate the integral as follows:

\[\oint\limits_{C}\mathrm{\frac{e^z}{(z-i)^2\cdot(z+2)}dz} = \oint\limits_{\mathrm{l_1}}\mathrm{\frac{e^z}{(z-i)^2\cdot(z+2)}dz}+ \oint\limits_{\mathrm{l_2}}\mathrm{\frac{e^z}{(z-i)^2\cdot(z+2)}dz}\]

where \(\mathrm{l_1}\) and \(\mathrm{l_2}\) are the contours contating only one of the roots. 
Let  \(\mathrm{l_1}\) be \(|z - i| = 1\), \(\mathrm{l_2}\) be \(|z+2| = 1\).

\[\oint\limits_{C}\mathrm{\frac{e^z}{(z-i)^2\cdot(z+2)}dz} = \oint\limits_{\mathrm{|z - i| = 1}}\mathrm{\frac{\frac{e^z}{z+2}}{(z-i)^2}dz}+ \oint\limits_{\mathrm{l_2}}\mathrm{\frac{\frac{e^z}{(z-i)^2}}{z-(-2)}dz} = \frac{2 \pi i}{1!}\cdot (\frac{e^z}{z+2})'|_{\mathrm{z=i}} + \frac{2 \pi i}{0!}\cdot (\frac{e^z}{(z-i)^2})|_{\mathrm{z=-2}} \]

\[
    = 2 \pi i \cdot \frac{e^i\cdot (i+1)}{(i+2)^2} + 2 \pi i \cdot \frac{e^-2}{(i+2)^2} = 
        \frac{2 \pi i}{(i+2)^2}\cdot(e^-2 + e^i\cdot(i+1))
\]


\end{document}
